tests/ll/icmp.ll
@@ -1,0 +1,43 @@
+define i1 @icmp_eq(i32 %x, i32 %y) {
+  %ans = icmp eq i32 %x, %y
+  ret i1 %ans
+}
+
+; ASSERT EQ: i1 1 = call i1 @icmp_eq(i32 0, i32 0)
+; ASSERT EQ: i1 0 = call i1 @icmp_eq(i32 0, i32 17)
+
+define i1 @icmp_ult(i32 %x, i32 %y) {
+  %ans = icmp ult i32 %x, %y
+  ret i1 %ans
+}
+
+; ASSERT EQ: i1 0 = call i1 @icmp_ult(i32 0, i32 0)
+; ASSERT EQ: i1 1 = call i1 @icmp_ult(i32 0, i32 17)
+
+
+define i1 @icmp_slt(i32 %x, i32 %y) {
+  %ans = icmp slt i32 %x, %y
+  ret i1 %ans
+}
+
+; ASSERT EQ: i1 0 = call i1 @icmp_slt(i32 0, i32 0)
+; ASSERT EQ: i1 1 = call i1 @icmp_slt(i32 0, i32 17)
+; ASSERT EQ: i1 1 = call i1 @icmp_slt(i32 -1, i32 17)
+; ASSERT EQ: i1 1 = call i1 @icmp_slt(i32 -25, i32 -17)
+
+
+define i1 @icmp_samesign_eq(i32 %x, i32 %y) {
+  %ans = icmp samesign eq i32 %x, %y
+  ret i1 %ans
+}
+
+; ASSERT EQ: i1 1 = call i1 @icmp_samesign_eq(i32 0, i32 0)
+; ASSERT EQ: i1 0 = call i1 @icmp_samesign_eq(i32 0, i32 17)
+; ASSERT POISON: call i1 @icmp_samesign_eq(i32 -1, i32 17)
+; ASSERT EQ: i1 0 = call i1 @icmp_samesign_eq(i32 -25, i32 -17)
+; ASSERT POISON: call i1 @icmp_samesign_eq(i32 -25, i32 17)
+
+
+
+
+
