src/rocq/Syntax/LLVMAst.v
@@ -395,7 +395,7 @@ Inductive exp : Set :=
 | EXP_Array           (t:T) (elts: list (T * exp))
 | EXP_Vector          (t:T) (elts: list (T * exp))
 | OP_IBinop           (iop:ibinop) (t:T) (v1:exp) (v2:exp)
-| OP_ICmp             (cmp:icmp)   (t:T) (v1:exp) (v2:exp)
+| OP_ICmp             (samesign:bool) (cmp:icmp)   (t:T) (v1:exp) (v2:exp)
 | OP_FBinop           (fop:fbinop) (fm:list fast_math) (t:T) (v1:exp) (v2:exp)
 | OP_FCmp             (cmp:fcmp)   (t:T) (v1:exp) (v2:exp)
 | OP_Conversion       (conv:conversion_type) (t_from:T) (v:exp) (t_to:T)
